Fir/Wasm/Concrete.lean
@@ -28,3 +28,4 @@ import Fir.Wasm.Concrete.ReuseMemoryCorrectness
 import Fir.Wasm.Concrete.ResetReuseCorrectness
 import Fir.Wasm.Concrete.GlobalCorrectness
 import Fir.Wasm.Concrete.ExternalCorrectness
+import Fir.Wasm.Concrete.FaultCorrectness
